theories/Eq/SSim0Theory.v
@@ -46,147 +46,7 @@ End SSim0Notations.
 Import CTreeNotations.
 Import EquNotations.
 Import SBisimNotations.
-
-Section ssim0_heterogenous_theory.
-  Arguments label: clear implicits.
-  Context {E F C D: Type -> Type} {X Y: Type}
-          {L: rel (@label E) (@label F)}
-          {HasStuck1: B0 -< C} {HasStuck2: B0 -< D}.
-  
-  Notation ss0 := (@ss0 E F C D X Y _ _).
-  Notation ssim0  := (@ssim0 E F C D X Y _ _).
-  Notation sst0 L := (coinduction.t (ss0 L)).
-  Notation ssbt0 L := (coinduction.bt (ss0 L)).
-  Notation ssT0 L := (coinduction.T (ss0 L)).
-
- (*|
-Strong simulation up-to [equ] is valid
-----------------------------------------
-|*)
-  Lemma equ_clos_sst0 : equ_clos <= (sst0 L).
-  Proof.
-    apply Coinduction; cbn.
-    intros R x y [x' y' x'' y'' EQ' EQ''] l z x'z.
-    rewrite EQ' in x'z.
-    destruct (EQ'' _ _ x'z) as (l' & ? & ? & ? & ?).
-    exists l', x0.
-    split.
-    - rewrite <- Equu; auto.
-    - split; auto.
-      eapply (f_Tf (ss0 L)).
-      econstructor; auto; auto.
-  Qed.
-
-  #[global] Instance equ_clos_sst0_goal {RR} :
-    Proper (equ eq ==> equ eq ==> flip impl) (sst0 L RR).
-  Proof.
-    cbn; intros ? ? eq1 ? ? eq2 H.
-    apply (ft_t equ_clos_sst0); econstructor; [eauto | | symmetry; eauto]; assumption.
-  Qed.
-
-  #[global] Instance equ_clos_sst0_ctx {RR} :
-    Proper (equ eq ==> equ eq ==> impl) (sst0 L RR).
-  Proof.
-    cbn; intros ? ? eq1 ? ? eq2 H.
-    apply (ft_t equ_clos_sst0); econstructor; [symmetry; eauto | | eauto]; assumption.
-  Qed.
-
-  #[global] Instance equ_ssbt0_closed_goal {r} :
-    Proper (equ eq ==> equ eq ==> flip impl) (ssbt0 L r).
-  Proof.
-    cbn. intros.
-    apply (fbt_bt equ_clos_sst0); econstructor; eauto.
-    now symmetry.
-  Qed.
-
-  #[global] Instance equ_ssbt0_closed_ctx {r} :
-    Proper (equ eq ==> equ eq ==> impl) (ssbt0 L r).
-  Proof.
-    cbn; intros.    
-    now rewrite H, H0 in H1.
-  Qed.
-
-  #[global] Instance equ_clos_ssT0_goal RR f :
-    Proper (equ eq ==> equ eq ==> flip impl) (ssT0 L f RR).
-  Proof.
-    cbn; intros ? ? eq1 ? ? eq2 H.
-    apply (fT_T equ_clos_sst0); econstructor; [eauto | | symmetry; eauto]; assumption.
-  Qed.
-
-  #[global] Instance equ_clos_ssT0_ctx RR f :
-    Proper (equ eq ==> equ eq ==> impl) (ssT0 L f RR).
-  Proof.
-    cbn; intros ? ? eq1 ? ? eq2 H.
-    apply (fT_T equ_clos_sst0); econstructor; [symmetry; eauto | | eauto]; assumption.
-  Qed.
-
-  #[global] Instance equ_clos_ssim0_goal :
-    Proper (equ eq ==> equ eq ==> flip impl) (ssim0 L).
-  Proof.
-    cbn; intros ? ? eq1 ? ? eq2 H.
-    apply (ft_t equ_clos_sst0); econstructor; [eauto | | symmetry; eauto]; assumption.
-  Qed.
-
-  #[global] Instance equ_clos_ssim0_ctx :
-    Proper (equ eq ==> equ eq ==> impl) (ssim0 L).
-  Proof.
-    cbn; intros ? ? eq1 ? ? eq2 H.
-    apply (ft_t equ_clos_sst0); econstructor; [symmetry; eauto | | eauto]; assumption.
-  Qed.
-
-  #[global] Instance equ_ss0_closed_goal {r} :
-    Proper (equ eq ==> equ eq ==> flip impl) (ss0 L r).
-  Proof.
-    intros t t' tt' u u' uu'; cbn; intros.
-    rewrite tt' in H0. apply H in H0 as (l' & ? & ? & ? & ?).
-    do 2 eexists; eauto. rewrite uu'. eauto.
-  Qed.
-
-  #[global] Instance equ_ss0_closed_ctx {r} :
-    Proper (equ eq ==> equ eq ==> impl) (ss0 L r).
-  Proof.
-    intros t t' tt' u u' uu'; cbn; intros.
-    rewrite <- tt' in H0. apply H in H0 as (l' & ? & ? & ? & ?).
-    do 2 eexists; eauto. rewrite <- uu'. eauto.
-  Qed.
-
-  (*|
-    stuck ctrees can be simulated by anything.
-    |*)
-  Lemma is_stuck_ss0 (R : rel _ _) (t : ctree E C X) (t': ctree F D Y):
-    is_stuck t -> ss0 L R t t'.
-  Proof.
-    repeat intro. now apply H in H0.
-  Qed.
-
-  Lemma is_stuck_ssim0 (t: ctree E C X) (t': ctree F D Y):
-    is_stuck t -> ssim0 L t t'.
-  Proof.
-    intros. step. now apply is_stuck_ss0.
-  Qed.
-
-  Lemma stuckD_ss0 (R : rel _ _) (t : ctree F D Y) : ss0 L R stuckD t.
-  Proof.
-    repeat intro. now apply stuckD_is_stuck in H.
-  Qed.
-
-  Lemma stuckD_ssim0 (t : ctree F D Y) : ssim0 L stuckD t.
-  Proof.
-    intros. step. apply stuckD_ss0.
-  Qed.
-  
-  Lemma spinD_ss0 (R : rel _ _) (t : ctree F D Y) `{HasTau: B1 -< C}: ss0 L R spinD t.
-  Proof.
-    repeat intro. now apply spinD_is_stuck in H.
-  Qed.
-
-  Lemma spinD_ssim0 : forall (t' : ctree F D Y) `{HasTau: B1 -< C},
-      ssim0 L spinD t'.
-  Proof.
-    intros. step. apply spinD_ss0.
-  Qed.
-
-End ssim0_heterogenous_theory.
+Import SSim0Notations.
 
 Section ssim0_homogenous_theory.
   Context {E C: Type -> Type} {X: Type}
@@ -319,7 +179,154 @@ Section ssim0_homogenous_theory.
 
 End ssim0_homogenous_theory.
 
-Import SSim0Notations.
+(*| Parametric theory of [ss0] with heterogenous [L] |*)
+Section ssim0_heterogenous_theory.
+  Arguments label: clear implicits.
+  Context {E F C D: Type -> Type} {X Y: Type}
+          {L: rel (@label E) (@label F)}
+          {HasStuck1: B0 -< C} {HasStuck2: B0 -< D}.
+  
+  Notation ss0 := (@ss0 E F C D X Y _ _).
+  Notation ssim0  := (@ssim0 E F C D X Y _ _).
+  Notation sst0 L := (coinduction.t (ss0 L)).
+  Notation ssbt0 L := (coinduction.bt (ss0 L)).
+  Notation ssT0 L := (coinduction.T (ss0 L)).
+
+  (*|
+   Strong simulation up-to [equ] is valid
+   ----------------------------------------
+  |*)
+  Lemma equ_clos_sst0 : equ_clos <= (sst0 L).
+  Proof.
+    apply Coinduction; cbn.
+    intros R x y [x' y' x'' y'' EQ' EQ''] l z x'z.
+    rewrite EQ' in x'z.
+    destruct (EQ'' _ _ x'z) as (l' & ? & ? & ? & ?).
+    exists l', x0.
+    split.
+    - rewrite <- Equu; auto.
+    - split; auto.
+      eapply (f_Tf (ss0 L)).
+      econstructor; auto; auto.
+  Qed.
+
+  #[global] Instance equ_clos_sst0_goal {RR} :
+    Proper (equ eq ==> equ eq ==> flip impl) (sst0 L RR).
+  Proof.
+    cbn; intros ? ? eq1 ? ? eq2 H.
+    apply (ft_t equ_clos_sst0); econstructor; [eauto | | symmetry; eauto]; assumption.
+  Qed.
+
+  #[global] Instance equ_clos_sst0_ctx {RR} :
+    Proper (equ eq ==> equ eq ==> impl) (sst0 L RR).
+  Proof.
+    cbn; intros ? ? eq1 ? ? eq2 H.
+    apply (ft_t equ_clos_sst0); econstructor; [symmetry; eauto | | eauto]; assumption.
+  Qed.
+
+  #[global] Instance equ_ssbt0_closed_goal {r} :
+    Proper (equ eq ==> equ eq ==> flip impl) (ssbt0 L r).
+  Proof.
+    cbn. intros.
+    apply (fbt_bt equ_clos_sst0); econstructor; eauto.
+    now symmetry.
+  Qed.
+
+  #[global] Instance equ_ssbt0_closed_ctx {r} :
+    Proper (equ eq ==> equ eq ==> impl) (ssbt0 L r).
+  Proof.
+    cbn; intros.    
+    now rewrite H, H0 in H1.
+  Qed.
+
+  #[global] Instance equ_clos_ssT0_goal RR f :
+    Proper (equ eq ==> equ eq ==> flip impl) (ssT0 L f RR).
+  Proof.
+    cbn; intros ? ? eq1 ? ? eq2 H.
+    apply (fT_T equ_clos_sst0); econstructor; [eauto | | symmetry; eauto]; assumption.
+  Qed.
+
+  #[global] Instance equ_clos_ssT0_ctx RR f :
+    Proper (equ eq ==> equ eq ==> impl) (ssT0 L f RR).
+  Proof.
+    cbn; intros ? ? eq1 ? ? eq2 H.
+    apply (fT_T equ_clos_sst0); econstructor; [symmetry; eauto | | eauto]; assumption.
+  Qed.
+
+  #[global] Instance equ_clos_ssim0_goal :
+    Proper (equ eq ==> equ eq ==> flip impl) (ssim0 L).
+  Proof.
+    cbn; intros ? ? eq1 ? ? eq2 H.
+    apply (ft_t equ_clos_sst0); econstructor; [eauto | | symmetry; eauto]; assumption.
+  Qed.
+
+  #[global] Instance equ_clos_ssim0_ctx :
+    Proper (equ eq ==> equ eq ==> impl) (ssim0 L).
+  Proof.
+    cbn; intros ? ? eq1 ? ? eq2 H.
+    apply (ft_t equ_clos_sst0); econstructor; [symmetry; eauto | | eauto]; assumption.
+  Qed.
+
+  #[global] Instance equ_ss0_closed_goal {r} :
+    Proper (equ eq ==> equ eq ==> flip impl) (ss0 L r).
+  Proof.
+    intros t t' tt' u u' uu'; cbn; intros.
+    rewrite tt' in H0. apply H in H0 as (l' & ? & ? & ? & ?).
+    do 2 eexists; eauto. rewrite uu'. eauto.
+  Qed.
+
+  #[global] Instance equ_ss0_closed_ctx {r} :
+    Proper (equ eq ==> equ eq ==> impl) (ss0 L r).
+  Proof.
+    intros t t' tt' u u' uu'; cbn; intros.
+    rewrite <- tt' in H0. apply H in H0 as (l' & ? & ? & ? & ?).
+    do 2 eexists; eauto. rewrite <- uu'. eauto.
+  Qed.
+
+  (*|
+    stuck ctrees can be simulated by anything.
+    |*)
+  Lemma is_stuck_ss0 (R : rel _ _) (t : ctree E C X) (t': ctree F D Y):
+    is_stuck t -> ss0 L R t t'.
+  Proof.
+    repeat intro. now apply H in H0.
+  Qed.
+
+  Lemma is_stuck_ssim0 (t: ctree E C X) (t': ctree F D Y):
+    is_stuck t -> ssim0 L t t'.
+  Proof.
+    intros. step. now apply is_stuck_ss0.
+  Qed.
+
+  Lemma stuckD_ss0 (R : rel _ _) (t : ctree F D Y) : ss0 L R stuckD t.
+  Proof.
+    repeat intro. now apply stuckD_is_stuck in H.
+  Qed.
+
+  Lemma stuckD_ssim0 (t : ctree F D Y) : ssim0 L stuckD t.
+  Proof.
+    intros. step. apply stuckD_ss0.
+  Qed.
+  
+  Lemma spinD_ss0 (R : rel _ _) (t : ctree F D Y) `{HasTau: B1 -< C}: ss0 L R spinD t.
+  Proof.
+    repeat intro. now apply spinD_is_stuck in H.
+  Qed.
+
+  Lemma spinD_ssim0 : forall (t' : ctree F D Y) `{HasTau: B1 -< C},
+      ssim0 L spinD t'.
+  Proof.
+    intros. step. apply spinD_ss0.
+  Qed.
+
+End ssim0_heterogenous_theory.
+
+#[global] Hint Resolve is_stuck_ss0: core.
+#[global] Hint Resolve is_stuck_ssim0: core.
+#[global] Hint Resolve stuckD_ss0: core.
+#[global] Hint Resolve stuckD_ssim0: core.
+#[global] Hint Resolve spinD_ss0: core.
+#[global] Hint Resolve spinD_ssim0: core.
 
 (*|
 Up-to [bind] context simulations
@@ -330,57 +337,61 @@ We now prove the same result, but for strong simulation.
 |*)
 
 Section bind.
+  Arguments label: clear implicits.
   Obligation Tactic := idtac.
 
-  Context {E C: Type -> Type} {X Y : Type}
-          {HasStuck: B0 -< C}.
-
-(*|
-Specialization of [bind_ctx] to a function acting with [ssim] on the bound value,
-and with the argument (pointwise) on the continuation.
-|*)
-  Program Definition bind_ctx_ssim0 : mon (rel (ctree E C Y) (ctree E C Y)) :=
-    {|body := fun R => @bind_ctx E E C C X X Y Y (ssim0 eq) (pointwise eq R) |}.
+  Context {E F C D: Type -> Type} {X X' Y Y': Type}
+          `{HasStuck : B0 -< C} `{HasStuck' : B0 -< D}
+          (L : hrel (@label E) (@label F)).
+  (*|
+    Specialization of [bind_ctx] to a function acting with [ssim] on the bound value,
+    and with the argument (pointwise) on the continuation.
+    |*)
+  Program Definition bind_ctx_ssim0: mon (rel (ctree E C X') (ctree F D Y')) :=
+    {|body := fun R => @bind_ctx E F C D X Y X' Y' (ssim0 L) (pointwise (fun x y => L (val x) (val y)) R) |}.
   Next Obligation.
     intros ?? H. apply leq_bind_ctx. intros ?? H' ?? H''.
     apply in_bind_ctx. apply H'. intros t t' HS. apply H, H'', HS.
   Qed.
 
-  (* LEF: Make parametric on `L` *)
-(*|
-The resulting enhancing function gives a valid up-to technique
-|*)
-  Lemma bind_ctx_ssim0_t :
-    bind_ctx_ssim0 <= (sst0 eq).
+  (*|
+    The resulting enhancing function gives a valid up-to technique
+  |*)
+  Lemma bind_ctx_ssim0_t: 
+    respects_val L ->
+    bind_ctx_ssim0 <= (sst0 L).
   Proof.
-    intro HL.
+    intros HL.
     apply Coinduction.
     intros R. apply (leq_bind_ctx _).
     intros t1 t2 tt k1 k2 kk.
     step in tt.
-    intros l u STEP.
-    apply trans_bind_inv in STEP as [(H & t' & STEP & EQ) | (v & STEPres & STEP)]; cbn in *.
-    - apply tt in STEP as (l' & u' & STEP & ? & EQ'); subst.
-      do 2 eexists; split.
-      + eapply trans_bind_l; eauto.
-      + split.
+    simpl; intros l u STEP; 
+      apply trans_bind_inv in STEP as [(H & t' & STEP & EQ) | (v & STEPres & STEP)];
+      cbn in *.
+    apply tt in STEP as (u' & l' & STEP & EQ' & ?).
+    do 2 eexists. split.
+    apply trans_bind_l; eauto.
+    + intro Hl. destruct Hl. apply HL in H0 as [_ ?]. specialize (H0 (Is_val _)). auto.
+    + split; auto.
         apply (fT_T equ_clos_sst0).
         econstructor; [exact EQ | | reflexivity].
-        apply (fTf_Tf (ss0 eq)).
+        apply (fTf_Tf (ss0 L)).
         apply in_bind_ctx; auto.
-        intros ? ? ->.
-        apply (b_T (ss0 eq)).
-        red in kk. red. red. now apply kk. reflexivity.
-    - apply tt in STEPres as (l' & u' & STEPres & ? & ?); subst.
+        intros ? ? ?.
+        apply (b_T (ss0 L)).
+        red in kk; cbn; now apply kk.
+    + apply tt in STEPres as (u' & ? & STEPres & EQ' & ?).
+      specialize (HL _ _ H) as [? _]. specialize (H0 (Is_val _)). destruct H0.
+      pose proof (trans_val_invT STEPres). subst.
       pose proof (trans_val_inv STEPres) as EQ.
       rewrite EQ in STEPres.
-      specialize (kk v v eq_refl).
-      apply kk in STEP as (l'' & u'' & STEP & ? & EQ''); subst; cbn in *.
-      do 2 eexists.
-      split.
-      + eapply trans_bind_r; cbn in *; eauto.
-      + split. eapply (id_T (ss0 eq)); auto.
-        reflexivity.
+      specialize (kk v x0 H). 
+      apply kk in STEP as (u'' & ? & STEP & EQ'' & ?); cbn in *.
+      do 2 eexists; split.
+      eapply trans_bind_r; eauto.
+      split; auto.
+      eapply (id_T (ss0 L)); auto.
   Qed.
 
 End bind.
@@ -388,59 +399,66 @@ End bind.
 (*|
 Expliciting the reasoning rule provided by the up-to principles.
 |*)
-Lemma sst_clo_bind (E C : Type -> Type) (X Y : Type) :
-  forall (t1 t2 : ctree E C X) (k1 k2 : X -> ctree E C Y) RR `{HasStuck: B0 -< C},
-		t1 ≲ t2 ->
-    (forall x, (sst0 eq RR) (k1 x) (k2 x)) ->
-    sst0 eq RR (t1 >>= k1) (t2 >>= k2)
-.
+Lemma sst0_clo_bind {E F C D: Type -> Type} {X Y X' Y': Type} {L: rel (@label E) (@label F)}
+      `{HasStuck: B0 -< C} `{HasStuck': B0 -< D}
+      (t1 : ctree E C X) (t2: ctree F D Y)
+      (k1 : X -> ctree E C X') (k2 : Y -> ctree F D Y') RR:
+  respects_val L ->
+  ssim0 L t1 t2 ->
+  (forall x y, (sst0 L RR) (k1 x) (k2 y)) ->
+  sst0 L RR (t1 >>= k1) (t2 >>= k2).
 Proof.
-  intros.
-  apply (ft_t (@bind_ctx_ssim0_t E C X Y _)).
-  apply in_bind_ctx; auto.
-  intros ? ? <-; auto.
+  intros RV ? ?.
+  apply (ft_t (@bind_ctx_ssim0_t E F C D X X' Y Y' _ _ L RV)).
+  apply in_bind_ctx; eauto.
+  intros ? ? ?; auto.
 Qed.
 
 (*|
 Specializing the congruence principle for [≲]
 |*)
-Lemma ssim0_clo_bind (E C: Type -> Type) (X Y : Type) :
-  forall (t1 t2 : ctree E C X) (k1 k2 : X -> ctree E C Y) `{HasStuck: B0 -< C},
-		t1 ≲ t2 ->
-    (forall x, k1 x ≲ k2 x) ->
-    t1 >>= k1 ≲ t2 >>= k2
-.
+Lemma ssim0_clo_bind {E F C D: Type -> Type} {X Y X' Y': Type}  {L: rel (@label E) (@label F)}
+      `{HasStuck: B0 -< C} `{HasStuck': B0 -< D}
+      (t1 : ctree E C X) (t2: ctree F D Y)
+      (k1 : X -> ctree E C X') (k2 : Y -> ctree F D Y'):
+  respects_val L ->
+  ssim0 L t1 t2 ->
+  (forall x y, ssim0 L (k1 x) (k2 y)) ->
+  ssim0 L (t1 >>= k1) (t2 >>= k2).
 Proof.
-  intros * EQ EQs.
-  apply (ft_t (@bind_ctx_ssim0_t E C X Y _)).
+  intros * RV EQ EQs.
+  apply (ft_t (@bind_ctx_ssim0_t E F C D X X' Y Y' _ _ L RV)).
   apply in_bind_ctx; auto.
-  intros ? ? <-; auto.
+  intros ? ? ?; auto.
   apply EQs.
 Qed.
 
 (*|
 And in particular, we can justify rewriting [≲] to the left of a [bind].
 |*)
-Lemma bind_ssim0_cong_gen {E C X Y} RR {HasStuck: B0 -< C}:
-  Proper (ssim0 eq ==> pointwise_relation X (sst0 eq RR) ==> sst0 eq RR) (@bind E C X Y).
-
+Lemma bind_ssim0_cong_gen {E C X X'} RR {HasStuck: B0 -< C}
+      {L: relation (@label E)} `{respects_val L}:
+  Proper (ssim0 L ==> (fun f g => forall x y, sst0 L RR (f x) (g y)) ==> sst0 L RR) (@bind E C X X').
 Proof.
-  repeat red; intros; eapply sst_clo_bind; eauto.
+  do 4 red; intros.
+  eapply sst0_clo_bind; auto.
 Qed.
 
+Check @bind_ctx_ssim0_t.
+Check @ss0.
 Ltac __upto_bind_ssim0 :=
   match goal with
-    |- @ssim0 ?E ?F ?C ?D ?X ?Y _ _ (CTree.bind (T := ?T) _ _) (CTree.bind (T := ?T') _ _) =>
+    |- @ssim0 ?E ?F ?C ?D ?X ?Y _ _ ?L (CTree.bind (T := ?T) _ _) (CTree.bind (T := ?T') _ _) =>
       apply ssim0_clo_bind
-  | |- body (t (@ss0 ?E ?F ?C ?D ?X ?Y _ _)) ?R (CTree.bind (T := ?T) _ _) (CTree.bind (T := ?T) _ _) =>
-      apply (ft_t (@bind_ctx_ssim0_t E C T X _)), in_bind_ctx
-  | |- body (bt (@ss0 ?E ?F ?C ?D ?X ?Y _ _)) ?R (CTree.bind (T := ?T) _ _) (CTree.bind (T := ?T) _ _) =>
-      apply (fbt_bt (@bind_ctx_ssim0_t E C T X _)), in_bind_ctx
+  | |- body (t (@ss0 ?E ?F ?C ?D ?X ?Y _ _ ?L)) ?R (CTree.bind (T := ?T) _ _) (CTree.bind (T := ?T') _ _) =>
+      apply (ft_t (@bind_ctx_ssim0_t E F C D X T Y T' _ L)), in_bind_ctx
+  | |- body (bt (@ss0 ?E ?F ?C ?D ?X ?Y _ _ ?L)) ?R (CTree.bind (T := ?T) _ _) (CTree.bind (T := ?T') _ _) =>
+      apply (fbt_bt (@bind_ctx_ssim0_t E F C D X T Y T' _ L)), in_bind_ctx
   end.
 
 Ltac __upto_bind_eq_ssim0 :=
   match goal with
-  | |- @ssim0 ?E ?F ?C ?D ?X ?Y _ _ (CTree.bind (T := ?T) _ _) (CTree.bind (T := ?T') _ _) =>
+  | |- @ssim0 ?E ?F ?C ?D ?X ?Y _ _ ?L (CTree.bind (T := ?T) _ _) (CTree.bind (T := ?T') _ _) =>
       __upto_bind_ssim0; [reflexivity | intros ?]
   | _ => __upto_bind_ssim0; [reflexivity | intros ? ? <-]
   end.
@@ -454,7 +472,7 @@ Ltac __play_ssim0_in H :=
 
 Ltac __eplay_ssim0 :=
   match goal with
-  | h : @ssim0 ?E _ ?C _ ?X _ _ _ ?L _ _ |- _ =>
+  | h : @ssim0 ?E ?F ?C ?D ?X ?Y _ _ ?L _ _ |- _ =>
       __play_ssim0_in h
   end.
 
@@ -464,48 +482,62 @@ Ltac __eplay_ssim0 :=
 
 Section Proof_Rules.
 
-  Context {E C: Type -> Type} {X Y : Type} {HasStuck: B0 -< C}.
+  Arguments label: clear implicits.
+  Context {E C: Type -> Type}
+          {X : Type}
+          {HasStuck: B0 -< C}.
 
-  Lemma step_ss0_ret_gen (x y : X) (R : rel _ _) :
+  Lemma step_ss0_ret_gen {Y F D} `{HasStuck': B0 -< D}(x : X) (y : Y) (R L : rel _ _) :
     R stuckD stuckD ->
     (Proper (equ eq ==> equ eq ==> impl) R) ->
-    x = y ->
-    ss0 eq R (Ret x : ctree E C X) (Ret y).
+    L (val x) (val y) ->
+    ss0 L R (Ret x : ctree E C X) (Ret y : ctree F D Y).
   Proof.
-    intros Rstuck PROP <-.
-    cbn; intros ? ? TR; inv_trans; subst.
-    cbn; do 2 eexists. 
-    split.
-    - etrans.
-    - split. now rewrite EQ. reflexivity.
+    intros Rstuck PROP Lval.
+    cbn; intros ? ? TR; inv_trans; subst;
+      cbn; eexists; eexists; intuition; etrans;
+      now rewrite EQ.
   Qed.
 
-  Lemma step_ss0_ret (x y : X) (R : rel _ _) :
-    x = y ->
-    ssbt0 eq R (Ret x : ctree E C X) (Ret y).
+  Lemma step_ss0_ret {Y F D} `{HasStuck': B0 -< D} (x : X) (y : Y) (R L : rel _ _) :
+    L (val x) (val y) ->
+    ssbt0 L R (Ret x : ctree E C X) (Ret y : ctree F D Y).
   Proof.
+    intros.
     apply step_ss0_ret_gen.
-    reflexivity.
-    typeclasses eauto.
+    - step. intros.
+      apply is_stuck_ss0; apply stuckD_is_stuck.
+    - typeclasses eauto.
+    - apply H.
   Qed.
 
   (*|
-    The vis nodes are deterministic from the perspective of the labeled transition system,
-    stepping is hence symmetric and we can just recover the itree-style rule.
-    |*)
-  Lemma step_ss0_vis_gen (e : E X) (k k' : X -> ctree E C Y) (R : rel _ _) :
+    The vis nodes are deterministic from the perspective of the labeled
+    transition system, stepping is hence symmetric and we can just recover
+    the itree-style rule.
+  |*)
+  (* LEF: Here, maybe it would be nice to
+     have [k: Z -> ctree E C X], [k': Z' -> ctree F D Y] then the precondition
+     becomes [forall x, exists y, R (k x) (k' y) /\ L (obs e x) (obs f y)] but that's hard
+     for the [step_ss0_vis] proof. *)
+  Lemma step_ss0_vis_gen {Y Z Z' F D} `{HasStuck': B0 -< D} (e : E Z) (f: F Z')
+        (k : Z -> ctree E C X) (k' : Z' -> ctree F D Y) (R L: rel _ _) :
     (Proper (equ eq ==> equ eq ==> impl) R) ->
-    (forall x, R (k x) (k' x)) ->
-    ss0 eq R (Vis e k) (Vis e k').
+    (forall x, exists y, R (k x) (k' y) /\ L (obs e x) (obs f y)) ->
+    ss0 L R (Vis e k) (Vis f k').
   Proof.
-    intros PR EQs.
-    intros ? ? TR; inv_trans; subst.
-    cbn; do 2 eexists; split; [etrans | split; [rewrite EQ; eauto|reflexivity]].
-  Qed.
+    intros.
+    cbn; intros ? ? TR; inv_trans; subst;
+      destruct (H0 x) as (x' & RR & LL);
+      cbn; eexists; eexists; intuition.
+    - rewrite EQ; eauto. 
+    - assumption.      
+  Qed.     
 
-  Lemma step_ss0_vis (e : E X) (k k' : X -> ctree E C Y) (R : rel _ _) :
-    (forall x, sst0 eq R (k x) (k' x)) ->
-    ssbt0 eq R (Vis e k) (Vis e k').
+  Lemma step_ss0_vis {Y Z F D} `{HasStuck': B0 -< D} (e : E Z) (f: F Z)
+        (k : Z -> ctree E C X) (k' : Z -> ctree F D Y) (R L : rel _ _) :
+    (forall x, exists y, sst0 L R (k x) (k' y) /\ L (obs e x) (obs f y)) ->
+    ssbt0 L R (Vis e k) (Vis f k').
   Proof.
     intros * EQ.
     apply step_ss0_vis_gen; auto.
@@ -515,19 +547,23 @@ Section Proof_Rules.
   (*|
     Same goes for visible tau nodes.
     |*)
-   Lemma step_ss0_step_gen (t t' : ctree E C X) (R : rel _ _) {HasTau: B1 -< C}:
+  Lemma step_ss0_step_gen {Y F D} `{HasTau: B1 -< C} `{HasStuck': B0 -< D} `{HasTau': B1 -< D}
+        (t : ctree E C X) (t': ctree F D Y) (R L: rel _ _):
     (Proper (equ eq ==> equ eq ==> impl) R) ->
+    L tau tau ->
     (R t t') ->
-    ss0 eq R (Step t) (Step t').
+    ss0 L R (Step t) (Step t').
   Proof.
-    intros PR EQs.
+    intros PR ? EQs.
     intros ? ? TR; inv_trans; subst.
-    cbn; do 2 eexists; split; [etrans | split; [rewrite EQ; eauto|reflexivity]].
+    cbn; do 2 eexists; split; [etrans | split; [rewrite EQ; eauto|assumption]].
   Qed.
 
-  Lemma step_ss0_step (t t' : ctree E C X) (R : rel _ _) {HasTau: B1 -< C}:
-    (sst0 eq R t t') ->
-    ssbt0 eq R (Step t) (Step t').
+  Lemma step_ss0_step {Y F D} `{HasStuck': B0 -< D} `{HasTau: B1 -< C} `{HasTau': B1 -< D}
+        (t: ctree E C X) (t': ctree F D Y) (R L : rel _ _) :
+    (sst0 L R t t') ->
+    L tau tau ->
+    ssbt0 L R (Step t) (Step t').
   Proof.
     intros. apply step_ss0_step_gen; auto.
     typeclasses eauto.
@@ -539,50 +575,58 @@ Section Proof_Rules.
     A useful special case is the one where the arity coincide and we simply use the identity
     in both directions. We can in this case have [n] rather than [2n] obligations.
     |*)
-  Lemma step_ss0_brS_gen Z (c : C Y) (c' : C Z) (k : Y -> ctree E C X) (k' : Z -> ctree E C X) (R : rel _ _) :
+  Lemma step_ss0_brS_gen {Z Z' Y F D} `{HasStuck': B0 -< D} (c : C Z) (d : D Z')
+        (k : Z -> ctree E C X) (k' : Z' -> ctree F D Y) (R L: rel _ _) :
     (Proper (equ eq ==> equ eq ==> impl) R) ->
     (forall x, exists y, R (k x) (k' y)) ->
-    ss0 eq R (BrS c k) (BrS c' k').
+    L tau tau ->
+    ss0 L R (BrS c k) (BrS d k').
   Proof.
-    intros PROP EQs ? ? TR; inv_trans; subst.
+    intros PROP EQs ? ? ? TR; inv_trans; subst.
     destruct (EQs x) as [y HR].
-    cbn; do 2 eexists; split; [etrans | split; [rewrite EQ; eauto|reflexivity]].
+    cbn; do 2 eexists; split; [etrans | split; [rewrite EQ; eauto|assumption]].
   Qed.
 
-  Lemma step_ss0_brS Z (c : C Y) (c' : C Z) (k : Y -> ctree E C X) (k' : Z -> ctree E C X) (R : rel _ _) :
-    (forall x, exists y, sst0 eq R (k x) (k' y)) ->
-    ssbt0 eq R (BrS c k) (BrS c' k').
+  Lemma step_ss0_brS {Z Z' Y F} (c : C Z) (c' : C Z')
+        (k : Z -> ctree E C X) (k' : Z' -> ctree F C Y) (R L: rel _ _) :
+    (forall x, exists y, sst0 L R (k x) (k' y)) ->
+    L tau tau ->
+    ssbt0 L R (BrS c k) (BrS c' k').
   Proof.
     intros.    
     apply step_ss0_brS_gen; auto.
     typeclasses eauto.
   Qed.
 
-  Lemma step_ss0_brS_id_gen (c : C Y) (k k' : Y -> ctree E C X) (R : rel _ _) :
+  Lemma step_ss0_brS_id_gen {Z Y D F} `{HasStuck': B0 -< D} (c : C Z) (d: D Z)
+        (k: Z -> ctree E C X) (k': Z -> ctree F D Y)(R L : rel _ _) :
     (Proper (equ eq ==> equ eq ==> impl) R) ->
-    (forall x, R (k x) (k' x)) ->
-    ss0 eq R (BrS c k) (BrS c k').
+    (forall x, exists y, R (k x) (k' y)) ->
+    L tau tau ->
+    ss0 L R (BrS c k) (BrS d k').
   Proof.
     intros; apply step_ss0_brS_gen; eauto.
   Qed.
   
-  Lemma step_ss0_brS_id (c : C Y) (k k' : Y -> ctree E C X) (R : rel _ _) :
-    (forall x, sst0 eq R (k x) (k' x)) ->
-    ssbt0 eq R (BrS c k) (BrS c k').
+  Lemma step_ss0_brS_id {Z Y F} (c : C Z)
+        (k: Z -> ctree E C X) (k': Z -> ctree F C Y)(R L : rel _ _) :
+    (forall x, exists y, sst0 L R (k x) (k' y)) ->
+    L tau tau ->
+    ssbt0 L R (BrS c k) (BrS c k').
   Proof.
     intros.
-    apply step_ss0_brS_id_gen.
+    apply step_ss0_brS_id_gen; eauto. 
     typeclasses eauto.
-    eauto.
   Qed.
 
   (*|
     For invisible nodes, the situation is different: we may kill them, but that execution
     cannot act as going under the guard.
     |*)
-  Lemma step_ss0_guard_gen (t t' : ctree E C X) (R : rel _ _) {HasTau: B1 -< C}:
-    ss0 eq R t t' ->
-    ss0 eq R (Guard t) (Guard t').
+  Lemma step_ss0_guard_gen {Y F D} `{HasStuck': B0 -< D} `{HasTau: B1 -< C} `{HasTau': B1 -< D}
+        (t: ctree E C X) (t': ctree F D Y) (R L: rel _ _):
+    ss0 L R t t' ->
+    ss0 L R (Guard t) (Guard t').
   Proof.
     intros EQ.
     intros ? ? TR; inv_trans; subst.
@@ -590,16 +634,18 @@ Section Proof_Rules.
     do 2 eexists; split; [etrans | split; trivial].
   Qed.
 
-  Lemma step_ss0_guard (t t' : ctree E C X) (R : rel _ _) {HasTau: B1 -< C} :
-    ssbt0 eq R t t' ->
-    ssbt0 eq R (Guard t) (Guard t').
+  Lemma step_ss0_guard {Y F D} `{HasStuck': B0 -< D} `{HasTau: B1 -< C} `{HasTau': B1 -< D}
+        (t: ctree E C X) (t': ctree F D Y) (R L: rel _ _):
+    ssbt0 L R t t' ->
+    ssbt0 L R (Guard t) (Guard t').
   Proof.
     apply step_ss0_guard_gen.
   Qed.
 
-  Lemma step_ss0_brD_l_gen n (c : C n) (k : n -> ctree E C X) (t': ctree E C X) (R: rel _ _):
-    (forall x, ss0 eq R (k x) t') ->
-    ss0 eq R (BrD c k) t'.
+  Lemma step_ss0_brD_l_gen {Y F D Z} `{HasStuck': B0 -< D} (c : C Z)
+        (k : Z -> ctree E C X) (t': ctree F D Y) (R L: rel _ _):
+    (forall x, ss0 L R (k x) t') ->
+    ss0 L R (BrD c k) t'.
   Proof.
     intros EQs.
     intros ? ? TR; inv_trans; subst.
@@ -607,71 +653,68 @@ Section Proof_Rules.
     eauto.
   Qed.
 
-  Lemma step_ss0_brD_l n (c : C n) 
-    (k : n -> ctree E C X) (t' : ctree E C X) (R : rel _ _) :
-    (forall x, ssbt0 eq R (k x) t') ->
-    ssbt0 eq R (BrD c k) t'.
+  Lemma step_ss0_brD_l {Y F D Z} `{HasStuck': B0 -< D} (c : C Z)
+        (k : Z -> ctree E C X) (t: ctree F D Y) (R L: rel _ _):
+    (forall x, ssbt0 L R (k x) t) ->
+    ssbt0 L R (BrD c k) t.
   Proof.
     apply step_ss0_brD_l_gen.
   Qed.
 
-  Lemma step_ss0_brD_r_gen n (c: C n) (k : n -> ctree E C X) (t: ctree E C X) x R:
-    ss0 eq R t (k x) ->
-    ss0 eq R t (BrD c k).
+  Lemma step_ss0_brD_r_gen {Y F D Z} `{HasStuck': B0 -< D} (c : D Z) x
+        (k : Z -> ctree F D Y) (t: ctree E C X) (R L: rel _ _):
+    ss0 L R t (k x) ->
+    ss0 L R t (BrD c k).
   Proof.
     cbn. intros.
     apply H in H0 as (? & ? & ? & ? & ?).
     exists x0; etrans.
   Qed.
 
-  Lemma step_ss0_brD_r n (c: C n) (k : n -> ctree E C X) (t: ctree E C X) x R:
-    ssbt0 eq R t (k x) ->
-    ssbt0 eq R t (BrD c k).
+  Lemma step_ss0_brD_r{Y F D Z} `{HasStuck': B0 -< D} (c : D Z) x
+        (k : Z -> ctree F D Y) (t: ctree E C X) (R L: rel _ _):
+    ssbt0 L R t (k x) ->
+    ssbt0 L R t (BrD c k).
   Proof.
     intros. eapply step_ss0_brD_r_gen. apply H.
   Qed.
 
-  Lemma step_ss0_brD_gen n m (cn: C n) (cm: C m)
-    (k : n -> ctree E C X) (k' : m -> ctree E C X) (R : rel _ _) :
-    (forall x, exists y, ss0 eq R (k x) (k' y)) ->
-    ss0 eq R (BrD cn k) (BrD cm k').
+  Lemma step_ss0_brD_gen {Y F D n m} `{HasStuck': B0 -< D} (a: C n) (b: D m)
+    (k : n -> ctree E C X) (k' : m -> ctree F D Y) (R L : rel _ _) :
+    (forall x, exists y, ss0 L R (k x) (k' y)) ->
+    ss0 L R (BrD a k) (BrD b k').
   Proof.
     intros EQs.
     apply step_ss0_brD_l_gen.
     intros. destruct (EQs x) as [x' ?].
-    now apply step_ss0_brD_r_gen with (x := x').
+    now apply step_ss0_brD_r_gen with (x:=x').
   Qed.
 
-  Lemma step_ss0_brD n m (cn: C n) (cm: C m)
-    (k : n -> ctree E C X) (k' : m -> ctree E C X) (R : rel _ _) :
-    (forall x, exists y, ssbt0 eq R (k x) (k' y)) ->
-    ssbt0 eq R (BrD cn k) (BrD cm k').
+  Lemma step_ss0_brD {Y F D n m} `{HasStuck': B0 -< D} (cn: C n) (cm: D m)
+    (k : n -> ctree E C X) (k' : m -> ctree F D Y) (L R : rel _ _) :
+    (forall x, exists y, ssbt0 L R (k x) (k' y)) ->
+    ssbt0 L R (BrD cn k) (BrD cm k').
   Proof.
     apply step_ss0_brD_gen.
   Qed.
 
-  Lemma step_ss0_brD_id_gen n (c: C n)
-    (k k' : n -> ctree E C X) (R : rel _ _) :
-    (forall x, ss0 eq R (k x) (k' x)) ->
-    ss0 eq R (BrD c k) (BrD c k').
+  Lemma step_ss0_brD_id_gen {Y F D n m} `{HasStuck': B0 -< D} (c: C n) (d: D m)
+        (k : n -> ctree E C X) (k' : m -> ctree F D Y)
+        (R L : rel _ _) :
+    (forall x, exists y, ss0 L R (k x) (k' y)) ->
+    ss0 L R (BrD c k) (BrD d k').
   Proof.
-    intros; apply step_ss0_brD_gen.
-    intros x; exists x; apply H.
+   intros; apply step_ss0_brD_gen.
+    intros x; destruct (H x) as [y ?]; exists y; apply H0.
   Qed.
 
-  Lemma step_ss0_brD_id n (c: C n)
-    (k k' : n -> ctree E C X) (R : rel _ _) :
-    (forall x, ssbt0 eq R (k x) (k' x)) ->
-    ssbt0 eq R (BrD c k) (BrD c k').
+  Lemma step_ss0_brD_id {Y F D n m} `{HasStuck': B0 -< D} (c: C n) (d: D m)
+    (k : n -> ctree E C X) (k': m -> ctree F D Y) (R L: rel _ _) :
+    (forall x, exists y, ssbt0 L R (k x) (k' y)) ->
+    ssbt0 L R (BrD c k) (BrD d k').
   Proof.
     apply step_ss0_brD_id_gen.
   Qed.
-
-End Proof_Rules.
-
-Section WithParams.
-
-  Context {E C: Type -> Type} {X : Type} {HasStuck: B0 -< C}.
 
   (*|
     Note that with visible schedules, nary-spins are equivalent only
@@ -680,11 +723,13 @@ Section WithParams.
     With invisible schedules, they are always equivalent: neither of them
     produce any challenge for the other.
   |*)
-  Lemma spinS_gen_nonempty : forall {Z X Y} (c: C X) (c': C Y) (x: X) (y: Y),
-      @spinS_gen E C Z X c ≲ @spinS_gen E C Z Y c'.
+  Lemma spinS_gen_nonempty : forall {Z Y D F} {L: rel (label E) (label F)} `{HasStuck': B0 -< D}
+                               (c: C X) (c': C Y) (x: X) (y: Y),
+      L tau tau ->
+      ssim0 L (@spinS_gen E C Z X c) (@spinS_gen F C Z Y c').
   Proof.
-    intros R.
-    coinduction S CIH; cbn; intros ? ? ? ? ? ? ? ? TR.
+    intros until L.
+    coinduction S CIH; simpl; intros ? ? ? ? ? ? ? ? TR;
       rewrite ctree_eta in TR; cbn in TR;
       apply trans_brS_inv in TR as (_ & EQ & ->);
       eexists; eexists;
@@ -694,69 +739,70 @@ Section WithParams.
       + reflexivity.
       + rewrite EQ; eauto.
   Qed.
-   
-
 
   (*|
     Inversion principles
     --------------------
     |*)
-  Lemma ssim0_ret_inv (r1 r2 : X) :
-    (Ret r1 : ctree E C X) ≲ Ret r2 ->
-    r1 = r2.
+  Lemma ssim0_ret_inv {F D} {L: rel (label E) (label F)} `{HasStuck': B0 -< D} (r1 r2 : X) :
+    ssim0 L (Ret r1 : ctree E C X) (Ret r2 : ctree F D X) ->
+    L (val r1) (val r2).
   Proof.
     intro.
     eplay.
-    destruct TR as (? & ? & ? & <-).
-    now inv_trans.    
+    destruct TR as (? & ? & ? & ?).    
+    inv_trans; subst; assumption.
   Qed.
-
-  Lemma ssim0_vis_inv_type {X1 X2}
-        (e1 : E X1) (e2 : E X2) (k1 : X1 -> ctree E C X) (k2 : X2 -> ctree E C X) (x : X1):
-    Vis e1 k1 ≲ Vis e2 k2 ->
+  
+  Lemma ssim0_vis_inv_type {D Y X1 X2} {L: relation (label E)} `{HasStuck': B0 -< D}
+        (e1 : E X1) (e2 : E X2) (k1 : X1 -> ctree E C X) (k2 : X2 -> ctree E D Y) (x : X1):
+    ssim0 L (Vis e1 k1) (Vis e2 k2) ->
     X1 = X2.
   Proof.
     intros.
     eplay.
-    destruct TR as (? & ? & ? & <-).
-    inv_trans. inv EQl; eauto.
-    Unshelve. exact x.
-  Qed.
-
-  Lemma ssbt0_eq_vis_inv {Y} (e1 e2 : E Y) (k1 k2 : Y -> ctree E C X) (x : Y) R :
-    ssbt0 eq R (Vis e1 k1) (Vis e2 k2) ->
-    e1 = e2 /\ forall x, sst0 eq R (k1 x) (k2 x).
-  Proof.
-    intros.
-    split.
-    - edestruct H as [? ? ?].
-      etrans. destruct H0 as (? & ? & ? & ?). subst. now inv_trans.
-    - intros.
-      edestruct H as [? ? ?].
-      etrans.
-      destruct H0 as (? & ? & ? & ?). subst. simpl in *.
-      inv H0. apply inj_pair2 in H4, H5,H6, H7; subst.
-      rewrite H3.
-      rewrite ctree_eta in H1; cbn in H1.
+    destruct TR as (? & ? & ? & ?).
+    inv_trans; subst; auto.
+    instantiate (1:=x) in H0.
   Admitted.
 
-  Lemma ssim0_eq_vis_inv {Y} (e1 e2 : E Y) (k1 k2 : Y -> ctree E C X) (x : Y) :
-    Vis e1 k1 ≲ Vis e2 k2 ->
-    e1 = e2 /\ forall x, k1 x ≲ k2 x.
+  Lemma ssbt0_vis_inv {F D Y X1 X2} {L: rel (label E) (label F)} `{HasStuck': B0 -< D}
+        (e1 : E X1) (e2 : F X2) (k1 : X1 -> ctree E C X) (k2 : X2 -> ctree F D Y) (x : X1) R:
+    ssbt0 L R (Vis e1 k1) (Vis e2 k2) ->
+    (exists y, L (obs e1 x) (obs e2 y))  /\ (forall x, exists y, sst0 L R (k1 x) (k2 y)).
   Proof.
     intros.
-    (* Why doesn't apply work directly here? *)
-    epose proof (proj1 (enhanced_gfp (@ss0 E E C C X X _ _ eq) _ _)). apply H0 in H. clear H0.
-    step in H. apply ssbt0_eq_vis_inv in H; auto.
-    destruct H. split; auto.
-    intro. subst. specialize (H0 x0).    
-    apply (proj1 (t_gfp_bt (@ss0 E E C C X X _ _ eq) _ _)) in H0. apply H0.
+    split; intros; edestruct H as [? ? ?];
+      etrans; subst; destruct H0 as (? & ? & ? & ? );
+      inv_trans; subst; eexists; auto.
+    - now eapply H2.
+    - now apply H1. 
   Qed.
 
-  Lemma ssim0_brS_inv
-        n m (cn: C n) (cm: C m) (k1 : n -> ctree E C X) (k2 : m -> ctree E C X) :
-    BrS cn k1 ≲ BrS cm k2 ->
-    (forall i1, exists i2, k1 i1 ≲ k2 i2).
+  Lemma ssim0_vis_inv {F D Y X1 X2} {L: rel (label E) (label F)} `{HasStuck': B0 -< D}
+        (e1 : E X1) (e2 : F X2) (k1 : X1 -> ctree E C X) (k2 : X2 -> ctree F D Y) (x : X1):
+    ssim0 L (Vis e1 k1) (Vis e2 k2) ->
+    (exists y, L (obs e1 x) (obs e2 y)) /\ (forall x, exists y, ssim0 L (k1 x) (k2 y)).
+  Proof.
+    intros.
+    split. 
+      - eplay; destruct TR as (? & ? & ? & ?).
+        inv_trans; subst; exists x2; eapply H1.
+      - epose proof (proj1 (enhanced_gfp (@ss0 E F C D X Y _ _ L) _ _)). apply H0 in H. clear H0.
+        step in H. eapply ssbt0_vis_inv in H.
+        destruct H as [[y Hy] ?].
+        intros.
+        destruct (H x0) as [y' Hy'].
+        eexists.
+        step.
+        econstructor; eexists; eauto; esplit.
+        + (* LEF: Because the left transitions doesn't mean the right will as well -- right could be stuck? *)
+   Admitted.        
+  
+  Lemma ssim0_brS_inv {F D Y} {L: rel (label E) (label F)} `{HasStuck': B0 -< D}
+        n m (cn: C n) (cm: D m) (k1 : n -> ctree E C X) (k2 : m -> ctree F D Y) :
+    ssim0 L (BrS cn k1) (BrS cm k2) ->
+    (forall i1, exists i2, ssim0 L (k1 i1) (k2 i2)).
   Proof.
     intros EQ i1.
     eplay.
@@ -765,10 +811,10 @@ Section WithParams.
     eexists; eauto.
   Qed.
 
-  Lemma ss0_brD_l_inv n (c: C n)
-    (t : ctree E C X) (k : n -> ctree E C X) R:
-    ss0 eq R (BrD c k) t ->
-    forall x, ss0 eq R (k x) t.
+  Lemma ss0_brD_l_inv {F D Y} {L: rel (label E) (label F)} `{HasStuck': B0 -< D}
+        n (c: C n) (t : ctree F D Y) (k : n -> ctree E C X) R:
+    ss0 L R (BrD c k) t ->
+    forall x, ss0 L R (k x) t.
   Proof.
     cbn. intros.
     eapply trans_brD in H0; [| reflexivity].
@@ -776,26 +822,26 @@ Section WithParams.
     eauto.
   Qed.
 
-  Lemma ssim0_brD_l_inv n (c: C n)
-    (t : ctree E C X) (k : n -> ctree E C X):
-    BrD c k ≲ t ->
-    forall x, k x ≲ t.
+  Lemma ssim0_brD_l_inv {F D Y} {L: rel (label E) (label F)} `{HasStuck': B0 -< D}
+        n (c: C n) (t : ctree F D Y) (k : n -> ctree E C X):
+    ssim0 L (BrD c k) t ->
+    forall x, ssim0 L (k x) t.
   Proof.
     intros. step. step in H. eapply ss0_brD_l_inv. apply H.
   Qed.
 
   (* This one isn't very convenient... *)
-  Lemma ssim0_brD_r_inv n (c: C n)
-    (t : ctree E C X) (k : n -> ctree E C X):
-    t ≲ BrD c k ->
+  Lemma ssim0_brD_r_inv {F D Y} {L: rel (label E) (label F)} `{HasStuck': B0 -< D}
+        n (c: D n) (t : ctree E C X) (k : n -> ctree F D Y):
+    ssim0 L t (BrD c k) ->
     forall l t', trans l t t' ->
-    exists x t'', trans l (k x) t'' /\ t' ≲ t''.
+    exists l' x t'' , trans l' (k x) t'' /\ L l l' /\ (ssim0 L t' t'').
   Proof.
     cbn. intros. step in H. apply H in H0 as (? & ? & ? & ? & ?); subst. inv_trans.
-    eauto.
+    do 3 eexists; eauto.
   Qed.
 
-End WithParams.
+End Proof_Rules.
 
 (*|
 A strong bisimulation gives two strong simulations,
@@ -824,7 +870,7 @@ Qed.
 #[local] Definition t2 : ctree void1 (B0 +' B1 +' B2) unit :=
   brS2 (Ret tt) (stuckD).
 
-Lemma ssim0_hsbisim_nequiv :
+Lemma ssim0_sbisim_nequiv :
   ssim0 eq t1 t2 /\ ssim0 eq t2 t1 /\ ~ sbisim eq t1 t2.
 Proof.
   unfold t1, t2. intuition.
