theories/Eq/SSimTheory.v
@@ -1,4 +1,8 @@
-From Coq Require Import Lia Basics Fin.
+From Coq Require Import
+     Lia
+     Basics
+     Fin
+     Logic.Eqdep.
 
 From Coinduction Require Import
      coinduction rel tactics.
@@ -19,8 +23,10 @@ From RelationAlgebra Require Export
 
 Set Implicit Arguments.
 
+Import CTree.
 Import EquNotations.
 Import SBisimNotations.
+Import CTreeNotations.
 
 (* TODO: Decide where to set this *)
 Arguments trans : simpl never.
@@ -30,7 +36,10 @@ Arguments trans : simpl never.
   __coinduction_sbisim R H || coinduction R H.
 #[local] Tactic Notation "step" "in" ident(H) := __step_in_sbisim H || step in H.
 
-
+(*| Very polymorphic definitions and lemmas
+  - Polymorphic on labels, by heterogenous relation [L].
+  - Polymorphic on return type.
+  - Polymorphic on branch effects. |*)
 Section ssim_heterogenous_theory.
   
   Arguments label: clear implicits.
@@ -47,12 +56,6 @@ Section ssim_heterogenous_theory.
 
   (*|
     Various results on reflexivity and transitivity.
-    |*)
-
-  (*|
-    Aggressively providing instances for rewriting hopefully faster
-    [sbisim] under relevant [ss]-related contexts (consequence of the transitivity
-    of the companion).
     |*)
   Lemma sbisim_clos_ss : @sbisim_clos E F C D X Y _ _ eq eq <= (sst L).
   Proof.
@@ -460,14 +463,12 @@ The resulting enhancing function gives a valid up-to technique
 
 End bind.
 
+(*| More lemmas about [bind] |*)
 Lemma bind_ctx_ssim_eq_t {E C T X} `{B0 -< C} :
-    (bind_ctx_ssim (X := T) (Y := T) eq : mon (relation (ctree E C X))) <= sst eq.
+  (bind_ctx_ssim (X := T) (Y := T) eq : mon (relation (ctree E C X))) <= sst eq.
 Proof.
   apply bind_ctx_ssim_t. red. intros. now subst.
 Qed.
-
-Import CTree.
-Import CTreeNotations.
 
 (*|
 Expliciting the reasoning rule provided by the up-to principles.
@@ -477,8 +478,7 @@ Lemma sst_clo_bind (E F C D: Type -> Type) `{B0 -< C} `{B0 -< D} (X X' Y Y' : Ty
 		t1 (≲L) t2 ->
     respects_val L ->
     (forall x y, L (val x) (val y) -> (sst L RR) (k1 x) (k2 y)) ->
-    sst L RR (t1 >>= k1) (t2 >>= k2)
-.
+    sst L RR (t1 >>= k1) (t2 >>= k2).
 Proof.
   intros.
   apply (ft_t (@bind_ctx_ssim_t E F C D X Y X' Y' _ _ L H2)).
@@ -515,6 +515,7 @@ Proof.
   intros; eapply sst_clo_bind; red in H2; eauto.
 Qed.
 
+(*| Ltac automation rule for [bind] and [ssim] |*)
 Ltac __upto_bind_ssim :=
   match goal with
     |- @ssim _ _ _ _ ?X ?X' _ _ _ (CTree.bind (T := ?T) _ _) (CTree.bind (T := ?T') _ _) =>
@@ -524,6 +525,7 @@ Ltac __upto_bind_ssim :=
   | |- body (bt (@ss ?E ?E ?C ?C ?X ?X _ _ eq)) ?R (CTree.bind (T := ?T) _ _) (CTree.bind (T := ?T) _ _) =>
       apply (fbt_bt (@bind_ctx_ssim_eq_t E C T X _)), in_bind_ctx
   end.
+
 Ltac __upto_bind_eq_ssim :=
   __upto_bind_ssim; [reflexivity | intros ? _ _].
 
@@ -531,7 +533,7 @@ Ltac __play_ssim := step; cbn; intros ? ? ?TR.
 
 Ltac __play_ssim_in H :=
   step in H;
-  cbn in H; edestruct H as (? & ? & ?TR & ?EQ & ?);
+  cbn in H; edestruct H as (? & ? & ? & ? & ? );
   clear H; subst; [etrans |].
 
 Ltac __eplay_ssim :=
@@ -544,13 +546,13 @@ Ltac __eplay_ssim :=
 #[local] Tactic Notation "play" "in" ident(H) := __play_ssim_in H.
 #[local] Tactic Notation "eplay" := __eplay_ssim.
 
-Section Proof_Rules.
-
+Section Proof_Rules_Heterogenous.
+  Arguments label: clear implicits.
   Context {E F C D : Type -> Type}.
   Context {HasStuck : B0 -< C} {HasStuck' : B0 -< D}.
   Context {HasTau : B1 -< C} {HasTau' : B1 -< D}.
   Context {X X' Y Y' : Type}.
-  Context {L : rel (@label E) (@label F)}.
+  Context {L : rel (label E) (label F)}.
 
   Lemma step_ss_ret_gen (x : X) (y : Y) (R : rel _ _) :
     R stuckD stuckD ->
@@ -563,456 +565,282 @@ Section Proof_Rules.
       cbn; eexists; eexists; intuition; etrans;
       now rewrite EQ.
   Qed.
-End Proof_Rules.
 
-Section Foo.
-   Context {E C : Type -> Type} {X : Type}
-          {L: relation (@label E)}
-          {HasStuck: B0 -< C}.
-   
-   Lemma step_ss_ret (x y : X) (R : rel _ _) `{Reflexive _ L}:
-     x = y ->
-     ssbt L R (Ret x : ctree E C X) (Ret y: ctree E C X).
-   Proof.
-     intros.
-     apply step_ss_ret_gen.
-     apply refl_sst; eauto.
-     typeclasses eauto.
-     subst; reflexivity.
+  Lemma step_ss_ret (x : X) (y : Y) (R : rel _ _) :
+    L (val x) (val y) ->
+    ssbt L R (Ret x : ctree E C X) (Ret y : ctree F D Y).
+  Proof.
+    intros.
+    apply step_ss_ret_gen.
+    - step. intros. apply ss_is_stuck; apply stuckD_is_stuck.
+    - typeclasses eauto.
+    - apply H.
   Qed.
-    
 
-(*|
-The vis nodes are deterministic from the perspective of the labeled transition system,
-stepping is hence symmetric and we can just recover the itree-style rule.
-|*)
-<<<<<<< HEAD
+  (*|
+    The vis nodes are deterministic from the perspective of the labeled
+    transition system, stepping is hence symmetric and we can just recover
+    the itree-style rule.
+  |*)
   Lemma step_ss_vis_gen (l : rel _ _) (e : E X) (k : X -> ctree E C Y) (k' : X -> ctree E D Y') (R : rel _ _) :
     (Proper (equ eq ==> equ eq ==> impl) R) ->
     (forall x, R (k x) (k' x)) ->
     (forall x, l (obs e x) (obs e x)) ->
     ss l R (Vis e k) (Vis e k').
   Proof.
-    intros PR EQs.
-    intros ? ? ? TR; inv_trans; subst.
-    cbn; eexists; eexists; intuition. rewrite EQ; auto.
+    split.
+    - apply step_ss0_vis_gen; auto.
+    - intros. inv_trans; subst; etrans.
   Qed.
 
-  Lemma step_ss_vis (l : rel _ _) (e : E X) (k : X -> ctree E C Y) (k' : X -> ctree E D Y') (R : rel _ _) :
+  Lemma step_ss_vis (l : rel _ _) (e : E X)
+        (k : X -> ctree E C Y) (k' : X -> ctree E D Y') (R : rel _ _) :
     (forall x, sst l R (k x) (k' x)) ->
     (forall x, l (obs e x) (obs e x)) ->
     ssbt l R (Vis e k) (Vis e k').
-=======
-  Lemma step_ss_vis_gen (e : E X) (k k' : X -> ctree E Y) (R : rel _ _) :
-    (Proper (equ eq ==> equ eq ==> impl) R) ->
-    (forall x, R (k x) (k' x)) ->
-    ss R (Vis e k) (Vis e k').
-  Proof.
-    split.
-    - apply step_ss0_vis_gen; auto.
-    - intros. inv_trans. etrans.
-    Unshelve. auto.
-  Qed.
-
-  Lemma step_ss_vis (e : E X) (k k' : X -> ctree E Y) (R : rel _ _) :
-    (forall x, sst R (k x) (k' x)) ->
-    ssbt R (Vis e k) (Vis e k').
->>>>>>> master
   Proof.
     intros * EQ.
     apply step_ss_vis_gen; auto.
     typeclasses eauto.
   Qed.
-
-(*|
-Same goes for visible tau nodes.
-|*)
-<<<<<<< HEAD
-   Lemma step_ss_tauV_gen (t : ctree E C X) (t' : ctree F D Y) (R : rel _ _) :
+  
+  (*|
+    Same goes for visible tau nodes.
+  |*)
+  
+  Lemma step_ss_step_gen (t : ctree E C X) (t' : ctree F D Y) (R : rel _ _) :
     (Proper (equ eq ==> equ eq ==> impl) R) ->
     (R t t') ->
     L tau tau ->
-    ss L R (tauV t) (tauV t').
+    ss L R (Step t) (Step t').
   Proof.
-    intros PR EQs.
-    intros ? ? ? TR; inv_trans; subst.
-    cbn; eexists; eexists; intuition; rewrite EQ; auto.
+    intros PR EQs ?.
+    cbn; split; intros ? ? TR; inv_trans; subst;
+      eexists; eexists; intuition.
+    - now rewrite EQ.
+    - assumption.
   Qed.
 
-  Lemma step_ss_tauV (t : ctree E C X) (t' : ctree F D Y) (R : rel _ _) :
+  Lemma step_ss_step (t : ctree E C X) (t' : ctree F D Y) (R : rel _ _) :
     L tau tau ->
     (sst L R t t') ->
-    ssbt L R (tauV t) (tauV t').
-  Proof.
-    intros. apply step_ss_tauV_gen; auto.
-=======
-   Lemma step_ss_step_gen (t t' : ctree E X) (R : rel _ _) :
-    (Proper (equ eq ==> equ eq ==> impl) R) ->
-    (R t t') ->
-    ss R (Step t) (Step t').
-  Proof.
-    split.
-    - apply step_ss0_step_gen; auto.
-    - etrans.
-  Qed.
-
-  Lemma step_ss_step (t t' : ctree E X) (R : rel _ _) :
-    (sst R t t') ->
-    ssbt R (Step t) (Step t').
+    ssbt L R (Step t) (Step t').
   Proof.
     intros. apply step_ss_step_gen; auto.
->>>>>>> master
     typeclasses eauto.
   Qed.
 
-(*|
-<<<<<<< HEAD
-When matching visible choices one against another, in general we need to explain how
-=======
-When matching visible brs one against another, in general we need to explain how
->>>>>>> master
-we map the branches from the left to the branches to the right.
-A useful special case is the one where the arity coincide and we simply use the identity
-in both directions. We can in this case have [n] rather than [2n] obligations.
-|*)
-<<<<<<< HEAD
+  (*|
+    When matching visible brs one against another, in general we need to explain how
+    we map the branches from the left to the branches to the right.
+    A useful special case is the one where the arity coincide and we simply use
+    the identity in both directions. We can in this case have [n] rather than [2n]
+    obligations.
+  |*)
 
-  Lemma step_ss_choiceV_gen C' Z `{C0 -< C'} (c : C Y) (c' : C' Z)
+  (** LEF: Here I need to show [Y] is inhabited,
+      I think the way to go is to axiomatize it. Maybe it's possible
+      to extract a [Y] from [HasTau: C]? *)
+  Lemma step_ss_brS_gen C' Z `{B0 -< C'} (c : C Y) (c' : C' Z)
     (k : Y -> ctree E C X) (k' : Z -> ctree F C' X') (R : rel _ _) :
     (Proper (equ eq ==> equ eq ==> impl) R) ->
     L tau tau ->
+    inhabited Y ->
     (forall x, exists y, R (k x) (k' y)) ->
-    ss L R (ChoiceV c k) (ChoiceV c' k').
+    ss L R (BrS c k) (BrS c' k').
   Proof.
-    intros PROP ? EQs.
-    intros ? ? TR; inv_trans; subst.
-    destruct (EQs x) as [z HR].
-    eexists. eexists. intuition.
-    rewrite EQ; eauto.
+    intros PROP ? EX EQs; cbn; split; 
+      intros ? ? TR; inv_trans; subst.
+    - destruct (EQs x) as [z HR].
+      do 2 eexists; intuition.      
+      rewrite EQ; eassumption.
+    - exists tau; eexists; intuition.
+      Unshelve. apply (proj1_sig EX).
   Qed.
 
-  Lemma step_ss_choiceV Z (c : C Y) (c' : D Z)
+  Lemma step_ss_brS Z (c : C Y) (c' : D Z)
     (k : Y -> ctree E C X) (k' : Z -> ctree F D X') (R : rel _ _) :
     L tau tau ->
+    inhabited Y ->
     (forall x, exists y, sst L R (k x) (k' y)) ->
-    ssbt L R (ChoiceV c k) (ChoiceV c' k').
+    ssbt L R (BrS c k) (BrS c' k').
   Proof.
-    intros ? EQs.
-    apply step_ss_choiceV_gen; auto.
-    typeclasses eauto.
-  Qed.
-
-  Lemma step_ss_choiceV_id_gen (c : C Y)
-    (k : Y -> ctree E C X) (k' : Y -> ctree F C X') (R : rel _ _) :
-    (Proper (equ eq ==> equ eq ==> impl) R) ->
-    L tau tau ->
-    (forall x, R (k x) (k' x)) ->
-    ss L R (ChoiceV c k) (ChoiceV c k').
-  Proof.
-    intros PROP ? EQs.
-    apply step_ss_choiceV_gen; auto.
-    intros x; exists x; auto.
-  Qed.
-
-  Lemma step_ss_choiceV_id (c : C Y)
-    (k : Y -> ctree E C X) (k' : Y -> ctree F C X') (R : rel _ _) :
-    L tau tau ->
-    (forall x, sst L R (k x) (k' x)) ->
-    ssbt L R (ChoiceV c k) (ChoiceV c k').
-  Proof.
-    apply step_ss_choiceV_id_gen.
-=======
-  Lemma step_ss_brS_gen n m (k : fin (S n) -> ctree E X) (k' : fin m -> ctree E X) (R : rel _ _) :
-    (Proper (equ eq ==> equ eq ==> impl) R) ->
-    (forall x, exists y, R (k x) (k' y)) ->
-    ss R (BrS (S n) k) (BrS m k').
-  Proof.
-    split.
-    - apply step_ss0_brS_gen; auto.
-    - etrans.
-    Unshelve. apply Fin.F1.
-  Qed.
-
-  Lemma step_ss_brS n m (k : fin (S n) -> ctree E X) (k' : fin m -> ctree E X) (R : rel _ _) :
-    (forall x, exists y, sst R (k x) (k' y)) ->
-    ssbt R (BrS (S n) k) (BrS m k').
-  Proof.
+    intros.
     apply step_ss_brS_gen; auto.
     typeclasses eauto.
   Qed.
 
-  Lemma step_ss_brS_id_gen n
-    (k k' : fin n -> ctree E X) (R : rel _ _) :
+  Lemma step_ss_brS_id_gen (c : C Y)
+    (k : Y -> ctree E C X) (k' : Y -> ctree F C X') (R : rel _ _) :
     (Proper (equ eq ==> equ eq ==> impl) R) ->
+    L tau tau ->
+    inhabited Y ->
     (forall x, R (k x) (k' x)) ->
-    ss R (BrS n k) (BrS n k').
+    ss L R (BrS c k) (BrS c k').
   Proof.
-    intros; destruct n.
-    - apply ss_is_stuck; rewrite br0_always_stuck; apply stuckS_is_stuck.
-    - apply step_ss_brS_gen; auto.
-      intros x; exists x; auto.
+    intros PROP ? ? EQs.
+    apply step_ss_brS_gen; auto.
+    intros x; exists x; auto.
   Qed.
 
-  Lemma step_ss_brS_id n
-    (k k' : fin n -> ctree E X) (R : rel _ _) :
-    (forall x, sst R (k x) (k' x)) ->
-    ssbt R (BrS n k) (BrS n k').
+  Lemma step_ss_brS_id (c : C Y)
+    (k : Y -> ctree E C X) (k' : Y -> ctree F C X') (R : rel _ _) :
+    L tau tau ->
+    inhabited Y ->
+    (forall x, sst L R (k x) (k' x)) ->
+    ssbt L R (BrS c k) (BrS c k').
   Proof.
     apply step_ss_brS_id_gen.
->>>>>>> master
     typeclasses eauto.
   Qed.
 
-(*|
-For invisible nodes, the situation is different: we may kill them, but that execution
-cannot act as going under the guard.
-|*)
-<<<<<<< HEAD
-  Lemma step_ss_tauI_gen (t : ctree E C X) (t' : ctree F D Y) (R : rel _ _) :
+  (*|
+    For invisible nodes, the situation is different: we may kill them, but that
+    execution cannot act as going under the guard.
+  |*)
+  Lemma step_ss_guard_gen (t : ctree E C X) (t' : ctree F D Y) (R : rel _ _) :
     ss L R t t' ->
-    ss L R (tauI t) (tauI t').
+    ss L R (Guard t) (Guard t').
   Proof.
-    intros EQ.
-    intros ? ? TR; inv_trans; subst.
-    apply EQ in TR as (? & ? & ? & ? & ?).
-    eexists; eexists; intuition; subst; [apply trans_tauI; eauto | eauto | eauto].
+    intros EQ; cbn; split; intros ? ? TR; inv_trans; subst.
+    - apply EQ in TR as (? & ? & ? & ? & ?).
+      do 2 eexists; intuition; subst; [apply trans_guard; eauto | eauto | eauto].
+    - apply EQ in TR as (? & ? & ? & ?).
+      do 2 eexists; subst; intuition.
+      + eapply H.
+      + apply trans_guard; eauto.
   Qed.
 
-  Lemma step_ss_tauI (t : ctree E C X) (t' : ctree F D Y) (R : rel _ _) :
+  Lemma step_ss_guard (t : ctree E C X) (t' : ctree F D Y) (R : rel _ _) :
     ssbt L R t t' ->
-    ssbt L R (tauI t) (tauI t').
-  Proof.
-    apply step_ss_tauI_gen.
-  Qed.
-
-  Lemma step_ss_choiceI_l_gen C' Z `{C0 -< C'} (c : C Z)
-    (k : Z -> ctree E C X) (t' : ctree F C' Y) (R : rel _ _) :
-    (forall x, ss L R (k x) t') ->
-    ss L R (ChoiceI c k) t'.
-  Proof.
-    intros EQs.
-    intros ? ? TR; inv_trans; subst.
-    apply EQs in TR; destruct TR as (u' & ? & TR' & EQ' & ?).
-    eexists. eexists. subst. intuition; eauto.
-  Qed.
-
-  Lemma step_ss_choiceI_l C' Z `{C0 -< C'} (c : C Z)
-    (k : Z -> ctree E C X) (t' : ctree F C' Y) (R : rel _ _) :
-    (forall x, ssbt L R (k x) t') ->
-    ssbt L R (ChoiceI c k) t'.
-  Proof.
-    apply step_ss_choiceI_l_gen.
-  Qed.
-
-  Lemma step_ss_choiceI_r_gen C' Z `{C0 -< C'} :
-    forall (t : ctree E C X) (c : C' Z) (k : Z -> ctree F C' Y) x R,
-    ss L R t (k x) ->
-    ss L R t (ChoiceI c k).
-  Proof.
-    simpl. intros.
-    apply H0 in H1 as (? & ? & ? & ? & ?). subst.
-    exists x0, x1. intuition. econstructor. eauto.
-  Qed.
-
-  Lemma step_ss_choiceI_r Z : forall (t : ctree E C X) (c : D Z) (k : Z -> ctree F D Y) x R,
-    ssbt L R t (k x) ->
-    ssbt L R t (ChoiceI c k).
-  Proof.
-    intros. eapply step_ss_choiceI_r_gen. apply H.
-  Qed.
-
-  Lemma step_ss_choiceI_gen C' Z Z' `{C0 -< C'} (c : C Z) (c' : C' Z')
-    (k : Z -> ctree E C X) (k' : Z' -> ctree F C' Y) (R : rel _ _) :
-    (forall x, exists y, ss L R (k x) (k' y)) ->
-    ss L R (ChoiceI c k) (ChoiceI c' k').
-  Proof.
-    intros EQs.
-    apply step_ss_choiceI_l_gen.
-    intros. destruct (EQs x) as [x' ?].
-    now apply step_ss_choiceI_r_gen with (x := x').
-  Qed.
-
-  Lemma step_ss_choiceI C' Z Z' `{C0 -< C'} (c : C Z) (c' : C' Z')
-    (k : Z -> ctree E C X) (k' : Z' -> ctree F C' Y) (R : rel _ _) :
-    (forall x, exists y, ssbt L R (k x) (k' y)) ->
-    ssbt L R (ChoiceI c k) (ChoiceI c' k').
-  Proof.
-    apply step_ss_choiceI_gen.
-  Qed.
-
-  Lemma step_ss_choiceI_id_gen Z (c : C Z)
-    (k : Z -> ctree E C X) (k' : Z -> ctree F C Y) (R : rel _ _) :
-    (forall x, ss L R (k x) (k' x)) ->
-    ss L R (ChoiceI c k) (ChoiceI c k').
-  Proof.
-    intros; apply step_ss_choiceI_gen.
-    intros x; exists x; apply H.
-  Qed.
-
-  Lemma step_ss_choiceI_id Z (c : C Z) (k : Z -> ctree E C X) (k' : Z -> ctree F C Y) (R : rel _ _) :
-    (forall x, ssbt L R (k x) (k' x)) ->
-    ssbt L R (ChoiceI c k) (ChoiceI c k').
-  Proof.
-    apply step_ss_choiceI_id_gen.
-=======
-  Lemma step_ss_guard_gen (t t' : ctree E X) (R : rel _ _) :
-    ss R t t' ->
-    ss R (Guard t) (Guard t').
-  Proof.
-    split.
-    - destruct H. apply step_ss0_tauI_gen. auto.
-    - intros. inv_trans.
-      apply H in H0 as (? & ? & ?).
-      etrans.
-  Qed.
-
-  Lemma step_ss_guard (t t' : ctree E X) (R : rel _ _) :
-    ssbt R t t' ->
-    ssbt R (Guard t) (Guard t').
+    ssbt L R (Guard t) (Guard t').
   Proof.
     apply step_ss_guard_gen.
   Qed.
 
-  Lemma step_ss_brD_l_gen n
-    (k : fin (S n) -> ctree E X) (t' : ctree E X) (R : rel _ _) :
-    (forall x, ss R (k x) t') ->
-    ss R (BrD (S n) k) t'.
+  Lemma step_ss_brD_l_gen C' Z `{B0 -< C'} (c : C Z)
+    (k : Z -> ctree E C X) (t' : ctree F C' Y) (R : rel _ _) :
+    (forall x, ss L R (k x) t') ->
+    inhabited Z -> 
+    ss L R (BrD c k) t'.
   Proof.
-    intros EQs. split.
-    - apply step_ss0_brD_l_gen. intro. now destruct (EQs x).
-    - intros. apply (EQs Fin.F1) in H as (? & ? & ?).
-      etrans.
+    intros EQs ?; cbn; split;
+      intros ? ? TR; inv_trans; subst.
+    - apply EQs in TR as (u' & ? & TR' & EQ' & ?); eauto.
+    - pose proof (proj1_sig X0) as z.
+      destruct (EQs z) as (tt & ? & ? & ? & ?); eauto.
+      do 2 eexists; intuition.
+      apply H0.
+      eapply trans_brD; eauto.
   Qed.
 
-  Lemma step_ss_brD_l n
-    (k : fin (S n) -> ctree E X) (t' : ctree E X) (R : rel _ _) :
-    (forall x, ssbt R (k x) t') ->
-    ssbt R (BrD (S n) k) t'.
+  Lemma step_ss_brD_l C' Z `{B0 -< C'} (c : C Z)
+    (k : Z -> ctree E C X) (t' : ctree F C' Y) (R : rel _ _) :
+    (forall x, ssbt L R (k x) t') ->
+    inhabited Z ->
+    ssbt L R (BrD c k) t'.
   Proof.
     apply step_ss_brD_l_gen.
   Qed.
 
-  Lemma step_ss_brD_r_gen :
-    forall (t : ctree E X) n (k : fin n -> ctree E X) x R,
-    (exists l t', trans l t t') ->
-    ss R t (k x) ->
-    ss R t (BrD n k).
+  Lemma step_ss_brD_r_gen C' Z `{B0 -< C'} :
+    forall (t : ctree E C X) (c : C' Z) (k : Z -> ctree F C' Y) x R,
+    ss L R t (k x) ->
+    ss L R t (BrD c k).
   Proof.
-    cbn. split; intros.
-    - apply H0 in H1 as [? ? ?].
-      exists x0; etrans.
-    - apply H.
+    simpl. split; intros.
+    - apply H0 in H1 as (? & ? & ? & ? & ?); subst.
+      exists x0, x1. intuition. econstructor. eauto.
+    - apply trans_brD_inv in H1 as (? & ?).
+      (** HM maybe this isn't so easy for complete simulation *)
+      admit.
+  Admitted.
+
+  Lemma step_ss_brD_r Z : forall (t : ctree E C X) (c : D Z) (k : Z -> ctree F D Y) x R,
+    ssbt L R t (k x) ->
+    ssbt L R t (BrD c k).
+  Proof.
+    intros. eapply step_ss_brD_r_gen. apply H.
   Qed.
 
-  Lemma step_ss_brD_r :
-    forall (t : ctree E X) n (k : fin n -> ctree E X) x R,
-    (exists l t', trans l t t') ->
-    ssbt R t (k x) ->
-    ssbt R t (BrD n k).
+  Lemma step_ss_brD_gen C' Z Z' `{B0 -< C'} (c : C Z) (c' : C' Z')
+    (k : Z -> ctree E C X) (k' : Z' -> ctree F C' Y) (R : rel _ _) :
+    (forall x, exists y, ss L R (k x) (k' y)) ->
+    inhabited Z ->
+    ss L R (BrD c k) (BrD c' k').
   Proof.
-    intros. eapply step_ss_brD_r_gen. apply H. apply H0.
+    intros EQs ?.
+    apply step_ss_brD_l_gen; trivial.
+    intros. destruct (EQs x) as [x' ?].
+    now apply step_ss_brD_r_gen with (x := x').
   Qed.
 
-  Lemma step_ss_brD_gen n m
-    (k : fin n -> ctree E X) (k' : fin m -> ctree E X) x (R : rel _ _) :
-    (exists l' t', trans l' (k x) t') ->
-    (forall x, exists y, ss R (k x) (k' y)) ->
-    ss R (BrD n k) (BrD m k').
-  Proof.
-    intros ? EQs. split; intros.
-    - apply step_ss0_brD_gen. intros.
-      destruct (EQs x0). destruct H0. eauto.
-    - destruct H as (? & ? & ?). etrans.
-  Qed.
-
-  Lemma step_ss_brD n m
-    (k : fin n -> ctree E X) (k' : fin m -> ctree E X) x (R : rel _ _) :
-    (exists l' t', trans l' (k x) t') ->
-    (forall x, exists y, ssbt R (k x) (k' y)) ->
-    ssbt R (BrD n k) (BrD m k').
+  Lemma step_ss_brD C' Z Z' `{B0 -< C'} (c : C Z) (c' : C' Z')
+    (k : Z -> ctree E C X) (k' : Z' -> ctree F C' Y) (R : rel _ _) :
+    (forall x, exists y, ssbt L R (k x) (k' y)) ->
+    inhabited Z -> 
+    ssbt L R (BrD c k) (BrD c' k').
   Proof.
     apply step_ss_brD_gen.
   Qed.
 
-  Lemma step_ss_brD_id_gen n
-    (k k' : fin n -> ctree E X) (R : rel _ _) :
-    (forall x, ss R (k x) (k' x)) ->
-    ss R (BrD n k) (BrD n k').
+  Lemma step_ss_brD_id_gen Z (c : C Z)
+    (k : Z -> ctree E C X) (k' : Z -> ctree F C Y) (R : rel _ _) :
+    (forall x, ss L R (k x) (k' x)) ->
+    inhabited Z ->
+    ss L R (BrD c k) (BrD c k').
   Proof.
-    destruct n; intros.
-    - apply ss_is_stuck; rewrite br0_always_stuck; apply stuckD_is_stuck.
-    - split; cbn; intros.
-      + inv_trans. apply H in TR as []. etrans.
-      + inv_trans. apply H in TR as (? & ? & ?). etrans.
+    intros; apply step_ss_brD_gen; trivial.
+    intros x; exists x; apply H.
   Qed.
 
-  Lemma step_ss_brD_id n
-    (k k' : fin n -> ctree E X) (R : rel _ _) :
-    (forall x, ssbt R (k x) (k' x)) ->
-    ssbt R (BrD n k) (BrD n k').
+  Lemma step_ss_brD_id Z (c : C Z) (k : Z -> ctree E C X) (k' : Z -> ctree F C Y) (R : rel _ _) :
+    (forall x, ssbt L R (k x) (k' x)) ->
+    inhabited Z -> 
+    ssbt L R (BrD c k) (BrD c k').
   Proof.
     apply step_ss_brD_id_gen.
->>>>>>> master
   Qed.
 
-End Proof_Rules.
+End Proof_Rules_Heterogenous.
 
 Section WithParams.
 
-<<<<<<< HEAD
   Context {E F C D : Type -> Type}.
-  Context {HasStuck : C0 -< C}.
-  Context {HasTau : C1 -< C}.
-  Context {HasStuck' : C0 -< D}.
-  Context {HasTau' : C1 -< D}.
+  Context {HasStuck : B0 -< C}.
+  Context {HasTau : B1 -< C}.
+  Context {HasStuck' : B0 -< D}.
+  Context {HasTau' : B1 -< D}.
   Context (L : rel (@label E) (@label F)).
-=======
-  Context {E : Type -> Type}.
-  Context {X : Type}.
->>>>>>> master
 
-(*|
-Note that with visible schedules, nary-spins are equivalent only
-if neither are empty, or if both are empty: they match each other's
-tau challenge infinitely often.
-With invisible schedules, they are always equivalent: neither of them
-produce any challenge for the other.
-|*)
-<<<<<<< HEAD
+  (*|
+    Note that with visible schedules, nary-spins are equivalent only
+    if neither are empty, or if both are empty: they match each other's
+    tau challenge infinitely often.
+    With invisible schedules, they are always equivalent: neither of them
+    produce any challenge for the other.
+    |*)
   Lemma spinV_gen_nonempty : forall {Z Z' X Y} (c: C X) (c': D Y) (x: X) (y: Y) (L : rel _ _),
     L tau tau ->
-    ssim L (@CTree.spinV_gen E C Z X c) (@CTree.spinV_gen F D Z' Y c').
+    ssim L (@spinS_gen E C Z X c) (@spinS_gen F D Z' Y c').
   Proof.
     intros.
     red. coinduction R CH.
-    intros l t' TR.
-    rewrite ctree_eta in TR; cbn in TR.
-    apply trans_choiceV_inv in TR as (_ & EQ & ->).
-    eexists. eexists.
-    rewrite ctree_eta; cbn.
-    split; [econstructor |]. exact y.
-    reflexivity.
-    rewrite EQ; auto.
-=======
-  Lemma spinS_nary_n_m : forall n m,
-    n > 0 -> m > 0 ->
-    ssim (@spinS_nary E X n) (spinS_nary m).
-  Proof.
-    intros.
-    red. coinduction R CH.
-    setoid_rewrite ctree_eta. cbn.
-    destruct n, m; try lia.
-    eapply step_ss_brS.
-    intros _. exists Fin.F1.
-    apply CH.
->>>>>>> master
+    simpl; split; intros l t' TR; rewrite ctree_eta in TR; cbn in TR;
+    apply trans_brS_inv in TR as (_ & EQ & ->);
+      do 2 eexists;
+      rewrite ctree_eta; cbn; intuition.
+    - econstructor; auto.
+    - rewrite EQ; eauto.
+    - eapply H.
+    - eapply H.
+    - econstructor; auto.
   Qed.
 
-(*|
-Inversion principles
---------------------
-|*)
-<<<<<<< HEAD
+  (*|
+    Inversion principles
+    --------------------
+  |*)
   Lemma ssim_ret_inv X Y (r1 : X) (r2 : Y) :
     (Ret r1 : ctree E C X) (≲L) (Ret r2 : ctree F D Y) ->
     L (val r1) (val r2).
@@ -1023,28 +851,18 @@ Inversion principles
 
   Lemma ssim_vis_inv_type {X X1 X2}
         (e1 : E X1) (e2 : E X2) (k1 : X1 -> ctree E C X) (k2 : X2 -> ctree E C X) (x : X1):
-=======
-  Lemma ssim_ret_inv (r1 r2 : X) :
-    (Ret r1 : ctree E X) ≲ Ret r2 ->
-    r1 = r2.
-  Proof.
-    intro.
-    eplay. etrans. inv_trans. auto.
-  Qed.
-
-  Lemma ssim_vis_inv_type {X1 X2}
-        (e1 : E X1) (e2 : E X2) (k1 : X1 -> ctree E X) (k2 : X2 -> ctree E X) (x : X1):
->>>>>>> master
     Vis e1 k1 ≲ Vis e2 k2 ->
     X1 = X2.
   Proof.
     intros.
     eplay.
-    inv TR; auto.
-    Unshelve. auto.
-  Qed.
-
-<<<<<<< HEAD
+    inv H2.
+    apply inj_pair2 in H6, H7; subst.
+    step in H1; inv H1; reflexivity.
+    Unshelve. admit.
+  Admitted.
+  (* Marker *)
+  
   Lemma ssbt_eq_vis_inv {X Y} (e1 e2 : E Y) (k1 k2 : Y -> ctree E C X) (x : Y) R :
     ss eq (t (ss eq) R) (Vis e1 k1) (Vis e2 k2) ->
     e1 = e2 /\ forall x, sst eq R (k1 x) (k2 x).
@@ -1053,22 +871,9 @@ Inversion principles
     split.
     - cbn in H. edestruct H as (? & ? & ? & ? & ?).
       etrans. subst. now inv_trans.
-    - cbn. intros. edestruct H as (? & ? & ? & ? & ?).
-=======
-  Lemma ssbt_eq_vis_inv {Y} (e1 e2 : E Y) (k1 k2 : Y -> ctree E X) (x : Y) R :
-    ssbt R (Vis e1 k1) (Vis e2 k2) ->
-    e1 = e2 /\ forall x, sst R (k1 x) (k2 x).
-  Proof.
-    intros. split.
-    - cbn in H. edestruct H as [[? ? ?] _].
-      etrans. subst. now inv_trans.
-    - cbn. intros. edestruct H as [[? ? ?] _].
->>>>>>> master
-      etrans. subst. inv_trans. subst. apply H1.
-    Unshelve. auto.
-  Qed.
+    - cbn. intros. edestruct H as [? ? ?].
+  Admitted.
 
-<<<<<<< HEAD
   Lemma t_gfp_bt : forall {X} `{CompleteLattice X} (b : mon X),
     weq (t b (gfp (bt b))) (gfp b).
   Proof.
@@ -1078,15 +883,11 @@ Inversion principles
   Qed.
 
   Lemma ssim_eq_vis_inv {X Y} (e1 e2 : E Y) (k1 k2 : Y -> ctree E C X) (x : Y) :
-=======
-  Lemma ssim_eq_vis_inv {Y} (e1 e2 : E Y) (k1 k2 : Y -> ctree E X) (x : Y) :
->>>>>>> master
     Vis e1 k1 ≲ Vis e2 k2 ->
     e1 = e2 /\ forall x, k1 x ≲ k2 x.
   Proof.
     intros.
     (* Why doesn't apply work directly here? *)
-<<<<<<< HEAD
     epose proof (proj1 (enhanced_gfp (@ss E E C C X X _ _ eq) _ _)). apply H0 in H. clear H0.
     step in H. apply ssbt_eq_vis_inv in H; auto.
     destruct H. split; auto.
@@ -1094,59 +895,45 @@ Inversion principles
     apply (proj1 (t_gfp_bt (@ss E E C C X X _ _ eq) _ _)) in H0. apply H0.
   Qed.
 
-  Lemma ssim_choiceV_inv {X Y Z Z'}
+  Lemma ssim_brS_inv {X Y Z Z'}
         c1 c2 (k1 : X -> ctree E C Z) (k2 : Y -> ctree F D Z') :
-    ChoiceV c1 k1 (≲L) ChoiceV c2 k2 ->
+    BrS c1 k1 (≲L) BrS c2 k2 ->
     (forall i1, exists i2, k1 i1 (≲L) k2 i2).
-=======
-    epose proof (proj1 (enhanced_gfp (@ss E X) _ _)). apply H0 in H. clear H0.
-    step in H. apply ssbt_eq_vis_inv in H; auto.
-    destruct H. split; auto.
-    intro. subst. specialize (H0 x0).
-    apply (proj1 (t_gfp_bt (@ss E X) _ _)) in H0. apply H0.
-  Qed.
-
-  Lemma ssim_brS_inv
-        n1 n2 (k1 : fin n1 -> ctree E X) (k2 : fin n2 -> ctree E X) :
-    BrS n1 k1 ≲ BrS n2 k2 ->
-    (forall i1, exists i2, k1 i1 ≲ k2 i2).
->>>>>>> master
   Proof.
-    intros EQ i1.
+    intros.
     eplay.
-    inv_trans.
-    eexists; eauto.
-  Qed.
+    inv_trans;
+      eexists; eauto.
+  Admitted.    
 
-<<<<<<< HEAD
-  Lemma ss_choiceI_l_inv : forall {X Y Z}
+  Lemma ss_brD_l_inv : forall {X Y Z}
     (t : ctree E C X) (c : D Y) (k : Y -> ctree F D Z) L R,
-    ss L R (ChoiceI c k) t ->
+    ss L R (BrD c k) t ->
     forall x, ss L R (k x) t.
   Proof.
-    cbn. intros.
-    eapply trans_choiceI in H0; [| reflexivity].
-    apply H in H0 as (? & ? & ? & ? & ?).
-    exists x0, x1. auto.
-  Qed.
+    cbn. intros; split; intros.
+    eapply trans_brD in H0; [| reflexivity].
+    - apply H in H0 as (? & ? & ? & ? & ?); exists x0, x1; auto.
+    - apply H in H0 as (? & ? & ? & ?). apply trans_brD_inv in H1 as (x' & y').
+  Admitted.
 
-  Lemma ssim_choiceI_l_inv : forall {X Y Z}
+  Lemma ssim_brD_l_inv : forall {X Y Z}
     (t : ctree E C X) (c : D Y) (k : Y -> ctree F D Z) L,
-    ChoiceI c k (≲L) t ->
+    BrD c k (≲L) t ->
     forall x, k x (≲L) t.
   Proof.
-    intros. step. step in H. eapply ss_choiceI_l_inv. apply H.
+    intros. step. step in H. eapply ss_brD_l_inv. apply H.
   Qed.
 
   (* This one isn't very convenient... *)
-  Lemma ssim_choiceI_r_inv : forall {X Y Z}
+  Lemma ssim_brD_r_inv : forall {X Y Z}
     (t : ctree E C X) (c : D Y) (k : Y -> ctree F D Z) L,
-    ssim L t (ChoiceI c k) ->
+    ssim L t (BrD c k) ->
     forall l t', trans l t t' ->
     exists x t'' l', trans l' (k x) t'' /\ ssim L t' t'' /\ L l l'.
   Proof.
     cbn. intros. step in H. apply H in H0 as (? & ? & ? & ? & ?). subst. inv_trans.
-    exists x1, x, x0. auto.
+    exists x1, x0, x. auto.
   Qed.
 
 End WithParams.
@@ -1158,16 +945,18 @@ This property is true if we only allow choices with 0 or 1 branch,
 but we prove a counter-example for a ctree with a binary choice.
 |*)
 
-Lemma ss_hsb : forall {E F C D X Y} `{C0 -< C} `{C0 -< D} L RR
+Lemma ss_sb : forall {E F C D X Y} `{B0 -< C} `{B0 -< D} L RR
   (t : ctree E C X) (t' : ctree F D Y),
   ss L RR t t' ->
   ss (flip L) (flip RR) t' t ->
-  hsb L RR t t'.
+  sb L RR t t'.
 Proof.
-  split; auto.
+  split; cbn; intros.
+  - apply H1 in H3 as (? & ? & ? & ? & ?); eauto.
+  - apply H2 in H3 as (? & ? & ? & ? & ?); eauto.
 Qed.
 
-Lemma ctree_C01_trans_det : forall {E X} l (t t' t'' : ctree E C01 X),
+Lemma ctree_B01_trans_det : forall {E X} l (t t' t'' : ctree E B01 X),
   trans l t t' -> trans l t t'' -> t' ≅ t''.
 Proof.
   intros. do 3 red in H.
@@ -1175,122 +964,80 @@ Proof.
   genobs t ot. genobs t' ot'. rewrite ctree_eta, <- Heqot'.
   clear t t' Heqot Heqot'. revert t'' H0.
   dependent induction H; intros; inv_trans.
-  - eapply IHtrans_; eauto.
+  - eapply IHtrans_; cbn.
     rewrite <- ctree_eta.
-    destruct c, c, x, x0. assumption.
-  - rewrite <- ctree_eta. destruct c, c, x, x0. now rewrite <- H, EQ.
+    destruct c, b, x0, x; intuition.
+  - rewrite <- ctree_eta. destruct c, b, x, x0.
+    now rewrite <- H, EQ.
   - subst. rewrite <- ctree_eta. now rewrite <- H, EQ.
-  - rewrite EQ. apply choice0_always_stuck.
-Qed.
+  - rewrite EQ. apply br0_always_stuck.
+Qed. 
 
-Lemma ssim_hsbisim_equiv_gen : forall {E F X Y} (L : rel _ _) (t : ctree E C01 X) (t' : ctree F C01 Y),
-  (forall x x' y, L x y -> L x' y -> x = x') ->
-  (forall x y y', L x y -> L x y' -> y = y') ->
-  ssim L t t' -> ssim (flip L) t' t -> hsbisim L t t'.
+
+Lemma ssim_sbisim_equiv_gen :
+  forall {E F X Y} (L : rel _ _) `{Injective _ _ L}
+    `{Deterministic _ _ L}
+    (t : ctree E B01 X) (t' : ctree F B01 Y),
+  ssim L t t' -> ssim (flip L) t' t -> sbisim L t t'.
 Proof.
-  intros until 2. revert t t'.
+  intros until 2.
   coinduction R CH. red. red. cbn. split; intros.
   - step in H1. cbn in H1.
     apply H1 in H3 as H3'. destruct H3' as (? & ? & ? & ? & ?).
     exists x, x0. intuition. apply CH.
     + apply H5.
     + step in H2. cbn in H2. apply H2 in H4 as (? & ? & ? & ? & ?).
-      replace x2 with l in H4.
-      2: { eapply H; eauto. }
-      assert (t'0 ≅ x1) by (eapply ctree_C01_trans_det; eauto).
-      now rewrite H9.
+      do_inj.
+      assert (t'0 ≅ x2) by (eapply ctree_B01_trans_det; eauto).
+      now rewrite H6.
   - step in H2. cbn in H2.
     apply H2 in H3 as H3'. destruct H3' as (? & ? & ? & ? & ?).
     exists x, x0. intuition. apply CH.
     + step in H1. cbn in H1. apply H1 in H4 as (? & ? & ? & ? & ?).
-      replace x2 with l in H4.
-      2: { eapply H0; eauto. }
-      assert (t'0 ≅ x1) by (eapply ctree_C01_trans_det; eauto).
-      now rewrite H9.
+      do_det.
+      assert (t'0 ≅ x2) by (eapply ctree_B01_trans_det; eauto).
+      now rewrite H6.
     + apply H5.
-Qed.
+  Qed.
 
-Lemma ssim_hsbisim_equiv : forall {E X} (t t' : ctree E C01 X),
-  ssim eq t t' -> ssim eq t' t -> hsbisim eq t t'.
+Lemma ssim_sbisim_equiv_eq : forall {E X} (t t' : ctree E B01 X),
+  ssim eq t t' -> ssim eq t' t -> sbisim eq t t'.
 Proof.
-  intros. apply ssim_hsbisim_equiv_gen; intros.
-  - now subst.
-  - now subst.
+  Print sb.
+  intros. apply ssim_sbisim_equiv_gen; intros.
+  - typeclasses eauto. 
+  - typeclasses eauto.
   - apply H.
-  - apply ssim_subrelation with (L := eq); auto.
+  - apply (@ssim_subrelation _ _ _ eq); auto.
     red. intros. subst. reflexivity.
 Qed.
 
-#[local] Definition t1 : ctree void1 (C01 +' C2) unit :=
-  tauV (Ret tt).
+#[local] Definition t1 : ctree void1 (B01 +' B2) unit :=
+  Step (Ret tt).
 
-#[local] Definition t2 : ctree void1 (C01 +' C2) unit :=
-  chooseV2 (Ret tt) (stuckI).
+#[local] Definition t2 : ctree void1 (B01 +' B2) unit :=
+  brS2 (Ret tt) (stuckD).
 
-Lemma ssim_hsbisim_nequiv :
-  ssim eq t1 t2 /\ ssim (flip eq) t2 t1 /\ ~ hsbisim eq t1 t2.
+Lemma ssim_sbisim_nequiv :
+  ssim eq t1 t2 /\ ssim (flip eq) t2 t1 /\ ~ sbisim eq t1 t2.
 Proof.
   unfold t1, t2. intuition.
-  - step. apply step_ss_choiceV; auto.
+  - step. eapply step_ss_brS; auto.
     intros _. exists true. reflexivity.
-  - step. apply step_ss_choiceV; auto.
+  - step. eapply step_ss_brS; auto.
     intro. exists tt. destruct x.
     + reflexivity.
-    + step. apply stuckI_ss.
+    + step. apply ss_is_stuck.
+      * apply stuckD_is_stuck.
+      * admit. (* This looks wrong, Ret is not stuck *)
   - step in H. cbn in H. destruct H as [_ ?].
-    specialize (H tau stuckI). lapply H; [| etrans].
+    specialize (H tau stuckD). lapply H; [| etrans].
     intros. destruct H0 as (? & ? & ? & ? & ?). subst.
     inv_trans. step in H1. cbn in H1. destruct H1 as [? _].
-    specialize (H0 (val tt) stuckI). lapply H0. 2: { rewrite EQ. etrans. }
+    specialize (H0 (val tt) stuckD). lapply H0. 2: { etrans. }
     intro. destruct H1 as (? & ? & ? & ? & ?). subst.
-    now apply stuckI_is_stuck in H1.
-Qed.
-=======
-  Lemma ss_brD_l_inv : forall n
-    (t : ctree E X) (k : fin n -> ctree E X) x R,
-    ss R (BrD n k) t ->
-    (exists l t', trans l (k x) t') ->
-    ss R (k x) t.
-  Proof.
-    split.
-    - apply ss0_brD_l_inv. now apply H.
-    - intros. apply H0.
-  Qed.
+    now apply stuckD_is_stuck in H1.
+    Unshelve. exact unit.
+    Unshelve. exact unit.
+Admitted.
 
-  Lemma ssim_brD_l_inv : forall n
-    (t : ctree E X) (k : fin n -> ctree E X) x,
-    BrD n k ≲ t ->
-    (exists l t', trans l (k x) t') ->
-    k x ≲ t.
-  Proof.
-    intros. step. step in H. eapply ss_brD_l_inv; auto.
-  Qed.
-
-  (* This one isn't very convenient... *)
-  Lemma ssim_brD_r_inv : forall n
-    (t : ctree E X) (k : fin n -> ctree E X),
-    t ≲ BrD n k ->
-    forall l t', trans l t t' ->
-    exists x t'', trans l (k x) t'' /\ t' ≲ t''.
-  Proof.
-    cbn. intros. step in H. apply H in H0 as [? ? ?]. inv_trans.
-    eauto.
-  Qed.
-
-End WithParams.
->>>>>>> master
-
-        
-Section ssim_heterogenous_theory.
-  #[local] Arguments label: clear implicits.
-  Context {E F C D : Type -> Type} {X Y : Type}
-          {L: rel (label E) (label F)}
-          {HasStuck1: B0 -< C} {HasStuck2: B0 -< D}.
-
-  Notation hss := (@ss E F C D X Y _ _ L).
-  Notation hssim  := (@ssim E F C D X Y _ _ L).
-  Notation hsst := (coinduction.t ss).
-  Notation hssbt := (coinduction.bt ss).
-  Notation hssT := (coinduction.T ss).
-  
-End ssim_heterogenous_theory.
